(*  Title:      HOL/Word/Bit_Lists.thy
    Author:     Jeremy Dawson, NICTA
*)

section \<open>Bit values as reversed lists of bools\<close>

theory Bit_Lists
  imports Bits_Int
begin

subsection \<open>Implicit augmentation of list prefixes\<close>

primrec takefill :: "'a \<Rightarrow> nat \<Rightarrow> 'a list \<Rightarrow> 'a list"
where
    Z: "takefill fill 0 xs = []"
  | Suc: "takefill fill (Suc n) xs =
      (case xs of
        [] \<Rightarrow> fill # takefill fill n xs
      | y # ys \<Rightarrow> y # takefill fill n ys)"

lemma nth_takefill: "m < n \<Longrightarrow> takefill fill n l ! m = (if m < length l then l ! m else fill)"
  apply (induct n arbitrary: m l)
   apply clarsimp
  apply clarsimp
  apply (case_tac m)
   apply (simp split: list.split)
  apply (simp split: list.split)
  done

lemma takefill_alt: "takefill fill n l = take n l @ replicate (n - length l) fill"
  by (induct n arbitrary: l) (auto split: list.split)

lemma takefill_replicate [simp]: "takefill fill n (replicate m fill) = replicate n fill"
  by (simp add: takefill_alt replicate_add [symmetric])

lemma takefill_le': "n = m + k \<Longrightarrow> takefill x m (takefill x n l) = takefill x m l"
  by (induct m arbitrary: l n) (auto split: list.split)

lemma length_takefill [simp]: "length (takefill fill n l) = n"
  by (simp add: takefill_alt)

lemma take_takefill': "n = k + m \<Longrightarrow> take k (takefill fill n w) = takefill fill k w"
  by (induct k arbitrary: w n) (auto split: list.split)

lemma drop_takefill: "drop k (takefill fill (m + k) w) = takefill fill m (drop k w)"
  by (induct k arbitrary: w) (auto split: list.split)

lemma takefill_le [simp]: "m \<le> n \<Longrightarrow> takefill x m (takefill x n l) = takefill x m l"
  by (auto simp: le_iff_add takefill_le')

lemma take_takefill [simp]: "m \<le> n \<Longrightarrow> take m (takefill fill n w) = takefill fill m w"
  by (auto simp: le_iff_add take_takefill')

lemma takefill_append: "takefill fill (m + length xs) (xs @ w) = xs @ (takefill fill m w)"
  by (induct xs) auto

lemma takefill_same': "l = length xs \<Longrightarrow> takefill fill l xs = xs"
  by (induct xs arbitrary: l) auto

lemmas takefill_same [simp] = takefill_same' [OF refl]

lemma tf_rev:
  "n + k = m + length bl \<Longrightarrow> takefill x m (rev (takefill y n bl)) =
    rev (takefill y m (rev (takefill x k (rev bl))))"
  apply (rule nth_equalityI)
   apply (auto simp add: nth_takefill rev_nth)
  apply (rule_tac f = "\<lambda>n. bl ! n" in arg_cong)
  apply arith
  done

lemma takefill_minus: "0 < n \<Longrightarrow> takefill fill (Suc (n - 1)) w = takefill fill n w"
  by auto

lemmas takefill_Suc_cases =
  list.cases [THEN takefill.Suc [THEN trans]]

lemmas takefill_Suc_Nil = takefill_Suc_cases (1)
lemmas takefill_Suc_Cons = takefill_Suc_cases (2)

lemmas takefill_minus_simps = takefill_Suc_cases [THEN [2]
  takefill_minus [symmetric, THEN trans]]

lemma takefill_numeral_Nil [simp]:
  "takefill fill (numeral k) [] = fill # takefill fill (pred_numeral k) []"
  by (simp add: numeral_eq_Suc)

lemma takefill_numeral_Cons [simp]:
  "takefill fill (numeral k) (x # xs) = x # takefill fill (pred_numeral k) xs"
  by (simp add: numeral_eq_Suc)


subsection \<open>Range projection\<close>

definition bl_of_nth :: "nat \<Rightarrow> (nat \<Rightarrow> 'a) \<Rightarrow> 'a list"
  where "bl_of_nth n f = map f (rev [0..<n])"

lemma bl_of_nth_simps [simp, code]:
  "bl_of_nth 0 f = []"
  "bl_of_nth (Suc n) f = f n # bl_of_nth n f"
  by (simp_all add: bl_of_nth_def)

lemma length_bl_of_nth [simp]: "length (bl_of_nth n f) = n"
  by (simp add: bl_of_nth_def)

lemma nth_bl_of_nth [simp]: "m < n \<Longrightarrow> rev (bl_of_nth n f) ! m = f m"
  by (simp add: bl_of_nth_def rev_map)

lemma bl_of_nth_inj: "(\<And>k. k < n \<Longrightarrow> f k = g k) \<Longrightarrow> bl_of_nth n f = bl_of_nth n g"
  by (simp add: bl_of_nth_def)

lemma bl_of_nth_nth_le: "n \<le> length xs \<Longrightarrow> bl_of_nth n (nth (rev xs)) = drop (length xs - n) xs"
  apply (induct n arbitrary: xs)
   apply clarsimp
  apply clarsimp
  apply (rule trans [OF _ hd_Cons_tl])
   apply (frule Suc_le_lessD)
   apply (simp add: rev_nth trans [OF drop_Suc drop_tl, symmetric])
   apply (subst hd_drop_conv_nth)
    apply force
   apply simp_all
  apply (rule_tac f = "\<lambda>n. drop n xs" in arg_cong)
  apply simp
  done

lemma bl_of_nth_nth [simp]: "bl_of_nth (length xs) ((!) (rev xs)) = xs"
  by (simp add: bl_of_nth_nth_le)

lemma takefill_bintrunc: "takefill False n bl = rev (bin_to_bl n (bl_to_bin (rev bl)))"
  apply (rule nth_equalityI)
   apply simp
  apply (clarsimp simp: nth_takefill rev_nth nth_bin_to_bl bin_nth_of_bl)
  done

lemma bl_bin_bl_rtf: "bin_to_bl n (bl_to_bin bl) = rev (takefill False n (rev bl))"
  by (simp add: takefill_bintrunc)


subsection \<open>More\<close>

definition rotater1 :: "'a list \<Rightarrow> 'a list"
  where "rotater1 ys =
    (case ys of [] \<Rightarrow> [] | x # xs \<Rightarrow> last ys # butlast ys)"

definition rotater :: "nat \<Rightarrow> 'a list \<Rightarrow> 'a list"
  where "rotater n = rotater1 ^^ n"

lemmas rotater_0' [simp] = rotater_def [where n = "0", simplified]

lemma rotate1_rl': "rotater1 (l @ [a]) = a # l"
  by (cases l) (auto simp: rotater1_def)

lemma rotate1_rl [simp] : "rotater1 (rotate1 l) = l"
  apply (unfold rotater1_def)
  apply (cases "l")
   apply (case_tac [2] "list")
    apply auto
  done

lemma rotate1_lr [simp] : "rotate1 (rotater1 l) = l"
  by (cases l) (auto simp: rotater1_def)

lemma rotater1_rev': "rotater1 (rev xs) = rev (rotate1 xs)"
  by (cases "xs") (simp add: rotater1_def, simp add: rotate1_rl')

lemma rotater_rev': "rotater n (rev xs) = rev (rotate n xs)"
  by (induct n) (auto simp: rotater_def intro: rotater1_rev')

lemma rotater_rev: "rotater n ys = rev (rotate n (rev ys))"
  using rotater_rev' [where xs = "rev ys"] by simp

lemma rotater_drop_take:
  "rotater n xs =
    drop (length xs - n mod length xs) xs @
    take (length xs - n mod length xs) xs"
  by (auto simp: rotater_rev rotate_drop_take rev_take rev_drop)

lemma rotater_Suc [simp]: "rotater (Suc n) xs = rotater1 (rotater n xs)"
  unfolding rotater_def by auto

lemma nth_rotater:
  \<open>rotater m xs ! n = xs ! ((n + (length xs - m mod length xs)) mod length xs)\<close> if \<open>n < length xs\<close>
  using that by (simp add: rotater_drop_take nth_append not_less less_diff_conv ac_simps le_mod_geq)

lemma nth_rotater1:
  \<open>rotater1 xs ! n = xs ! ((n + (length xs - 1)) mod length xs)\<close> if \<open>n < length xs\<close>
  using that nth_rotater [of n xs 1] by simp

lemma rotate_inv_plus [rule_format]:
  "\<forall>k. k = m + n \<longrightarrow> rotater k (rotate n xs) = rotater m xs \<and>
    rotate k (rotater n xs) = rotate m xs \<and>
    rotater n (rotate k xs) = rotate m xs \<and>
    rotate n (rotater k xs) = rotater m xs"
  by (induct n) (auto simp: rotater_def rotate_def intro: funpow_swap1 [THEN trans])

lemmas rotate_inv_rel = le_add_diff_inverse2 [symmetric, THEN rotate_inv_plus]

lemmas rotate_inv_eq = order_refl [THEN rotate_inv_rel, simplified]

lemmas rotate_lr [simp] = rotate_inv_eq [THEN conjunct1]
lemmas rotate_rl [simp] = rotate_inv_eq [THEN conjunct2, THEN conjunct1]

lemma rotate_gal: "rotater n xs = ys \<longleftrightarrow> rotate n ys = xs"
  by auto

lemma rotate_gal': "ys = rotater n xs \<longleftrightarrow> xs = rotate n ys"
  by auto

lemma length_rotater [simp]: "length (rotater n xs) = length xs"
  by (simp add : rotater_rev)

lemma rotate_eq_mod: "m mod length xs = n mod length xs \<Longrightarrow> rotate m xs = rotate n xs"
  apply (rule box_equals)
    defer
    apply (rule rotate_conv_mod [symmetric])+
  apply simp
  done

lemma restrict_to_left: "x = y \<Longrightarrow> x = z \<longleftrightarrow> y = z"
  by simp

lemmas rotate_eqs =
  trans [OF rotate0 [THEN fun_cong] id_apply]
  rotate_rotate [symmetric]
  rotate_id
  rotate_conv_mod
  rotate_eq_mod

lemmas rrs0 = rotate_eqs [THEN restrict_to_left,
  simplified rotate_gal [symmetric] rotate_gal' [symmetric]]
lemmas rrs1 = rrs0 [THEN refl [THEN rev_iffD1]]
lemmas rotater_eqs = rrs1 [simplified length_rotater]
lemmas rotater_0 = rotater_eqs (1)
lemmas rotater_add = rotater_eqs (2)

lemma butlast_map: "xs \<noteq> [] \<Longrightarrow> butlast (map f xs) = map f (butlast xs)"
  by (induct xs) auto

lemma rotater1_map: "rotater1 (map f xs) = map f (rotater1 xs)"
  by (cases xs) (auto simp: rotater1_def last_map butlast_map)

lemma rotater_map: "rotater n (map f xs) = map f (rotater n xs)"
  by (induct n) (auto simp: rotater_def rotater1_map)

lemma but_last_zip [rule_format] :
  "\<forall>ys. length xs = length ys \<longrightarrow> xs \<noteq> [] \<longrightarrow>
    last (zip xs ys) = (last xs, last ys) \<and>
    butlast (zip xs ys) = zip (butlast xs) (butlast ys)"
  apply (induct xs)
   apply auto
     apply ((case_tac ys, auto simp: neq_Nil_conv)[1])+
  done

lemma but_last_map2 [rule_format] :
  "\<forall>ys. length xs = length ys \<longrightarrow> xs \<noteq> [] \<longrightarrow>
    last (map2 f xs ys) = f (last xs) (last ys) \<and>
    butlast (map2 f xs ys) = map2 f (butlast xs) (butlast ys)"
  apply (induct xs)
   apply auto
     apply ((case_tac ys, auto simp: neq_Nil_conv)[1])+
  done

lemma rotater1_zip:
  "length xs = length ys \<Longrightarrow>
    rotater1 (zip xs ys) = zip (rotater1 xs) (rotater1 ys)"
  apply (unfold rotater1_def)
  apply (cases xs)
   apply auto
   apply ((case_tac ys, auto simp: neq_Nil_conv but_last_zip)[1])+
  done

lemma rotater1_map2:
  "length xs = length ys \<Longrightarrow>
    rotater1 (map2 f xs ys) = map2 f (rotater1 xs) (rotater1 ys)"
  by (simp add: rotater1_map rotater1_zip)

lemmas lrth =
  box_equals [OF asm_rl length_rotater [symmetric]
                 length_rotater [symmetric],
              THEN rotater1_map2]

lemma rotater_map2:
  "length xs = length ys \<Longrightarrow>
    rotater n (map2 f xs ys) = map2 f (rotater n xs) (rotater n ys)"
  by (induct n) (auto intro!: lrth)

lemma rotate1_map2:
  "length xs = length ys \<Longrightarrow>
    rotate1 (map2 f xs ys) = map2 f (rotate1 xs) (rotate1 ys)"
  by (cases xs; cases ys) auto

lemmas lth = box_equals [OF asm_rl length_rotate [symmetric]
  length_rotate [symmetric], THEN rotate1_map2]

lemma rotate_map2:
  "length xs = length ys \<Longrightarrow>
    rotate n (map2 f xs ys) = map2 f (rotate n xs) (rotate n ys)"
  by (induct n) (auto intro!: lth)

end
